CC/Subst.lean
@@ -10,20 +10,74 @@ import CC.Subtype
 import CC.Term
 import CC.Typed.Rename
 import CC.Subtype.Rename
+import CC.Subcapt.Rename
 
 namespace CC
 
+inductive SubcaptR : Ctx n m -> Region n -> CaptureSet n -> Prop where
+| scr_glob : SubcaptR Γ Region.glob C
+| scr_var :
+  Subcapt Γ ⟨∅, {x}, false⟩ C ->
+  SubcaptR Γ (Region.var x) C
+
+theorem SubcaptR.rename
+  (h : SubcaptR Γ r C)
+  (σ : VarRename Γ Δ f g) :
+  SubcaptR Δ (r.rename f) (C.rename f) := by
+  cases h
+  case scr_glob =>
+    constructor
+  case scr_var h =>
+    apply scr_var
+    have h' := h.rename σ
+    exact h'
+
+theorem SubcaptR.weaken_var (h : SubcaptR Γ r C) P p :
+  SubcaptR (Ctx.extend_var Γ P p) r.weaken_var C.weaken_var := by
+  apply SubcaptR.rename
+  exact h
+  apply VarRename.weaken_var_map
+
+theorem SubcaptR.weaken_tvar (h : SubcaptR Γ r C) P :
+  SubcaptR (Ctx.extend_tvar Γ P) r C := by
+  have heq1 : r.rename id = r := by simp [Region.rename_id]
+  have heq2 : C.rename id = C := by simp [CaptureSet.rename]
+  rw [<- heq1, <- heq2]
+  apply SubcaptR.rename
+  exact h
+  apply VarRename.weaken_tvar_map
+
+theorem SubcaptR.from_bound_var
+  (hb : BoundVar Γ x T r) :
+  SubcaptR Γ r ⟨∅, {x}, false⟩ := by
+  induction hb
+  case here r =>
+    cases r
+    case glob => constructor
+    case var =>
+      apply scr_var
+      apply Subcapt.sc_region
+      constructor
+  case there_var P p _ ih =>
+    have ih' := ih.weaken_var P p
+    exact ih'
+  case there_tvar P _ ih =>
+    have ih' := ih.weaken_tvar P
+    exact ih'
+
 def VarSubst (Γ : Ctx n1 m) (Δ : Ctx n2 m) (f : VarMap n1 n2) : Prop :=
-  ∀ {x T}, BoundVar Γ x T -> Typed Δ (Term.var (f x)) {f x} (T.rename f id)
+  ∀ {x T r}, BoundVar Γ x T r ->
+    Typed Δ (Term.var (f x)) {f x} (T.rename f id) ∧
+     SubcaptR Δ (r.rename f) ⟨∅, {f x}, false⟩
 
 def TVarSubst (Γ : Ctx n m1) (Δ : Ctx n m2) (g : TypeMap n m1 m2) : Prop :=
   ∀ {X S}, BoundTVar Γ X S -> SubtypeP Δ (g X) (S.tsubst g)
 
 def VarTypeMap (Γ : Ctx n m1) (Δ : Ctx n m2) (g : TypeMap n m1 m2) : Prop :=
-  ∀ {x T}, BoundVar Γ x T -> BoundVar Δ x (T.tsubst g)
+  ∀ {x T r}, BoundVar Γ x T r -> BoundVar Δ x (T.tsubst g) r
 
 theorem Typed.var_bound_type :
-  BoundVar Γ x T ->
+  BoundVar Γ x T r ->
   Typed Γ (Term.var x) {x} T := by
   intro hb
   cases T
@@ -36,35 +90,48 @@ theorem Typed.var_bound_type :
     constructor
 
 def VarSubst.ext_var (σ : VarSubst Γ Δ f) P :
-  VarSubst (Ctx.extend_var Γ P) (Ctx.extend_var Δ (P.rename f id)) f.ext := by
-  intros x T h
+  VarSubst (Ctx.extend_var Γ P p) (Ctx.extend_var Δ (P.rename f id) (p.rename f)) f.ext := by
+  intros x T r h
   cases h
   case here =>
-    conv =>
-      arg 2
-      simp [VarMap.ext]
-    conv =>
-      arg 3
-      simp [VarMap.ext]
-    rw [<- CType.rename_weaken_comm]
-    apply Typed.var_bound_type
-    constructor
+    apply And.intro
+    · conv =>
+        arg 2
+        simp [VarMap.ext]
+      conv =>
+        arg 3
+        simp [VarMap.ext]
+      rw [<- CType.rename_weaken_comm]
+      apply Typed.var_bound_type
+      constructor
+    · simp
+      rw [<- Region.rename_weaken_comm]
+      apply SubcaptR.from_bound_var
+      constructor
   case there_var h =>
-    conv =>
-      arg 2
-      simp [VarMap.ext]
-    conv =>
-      arg 3
-      simp [VarMap.ext]
-    rw [<- CType.rename_weaken_comm]
-    have h' := σ h
-    have h'' := h'.weaken_var (P.rename f id)
-    exact h''
+    apply And.intro
+    case left =>
+      conv =>
+        arg 2
+        simp [VarMap.ext]
+      conv =>
+        arg 3
+        simp [VarMap.ext]
+      rw [<- CType.rename_weaken_comm]
+      have ⟨h', _⟩ := σ h
+      have h'' := h'.weaken_var (P.rename f id)
+      apply h''
+    case right =>
+      simp [ext_succ]
+      rw [<- Region.rename_weaken_comm]
+      have ⟨_, h'⟩ := σ h
+      have h'' := h'.weaken_var (P.rename f id)
+      apply h''
 
 def VarTypeMap.ext_var
   (σ : VarTypeMap Γ Δ g) T :
-  VarTypeMap (Ctx.extend_var Γ T) (Ctx.extend_var Δ (T.tsubst g)) g.ext_var := by
-  intros x T h
+  VarTypeMap (Ctx.extend_var Γ T r) (Ctx.extend_var Δ (T.tsubst g) r) g.ext_var := by
+  intros x T r h
   cases h
   case here =>
     rw [CType.tsubst_weaken_var_comm]
@@ -78,7 +145,7 @@ def VarTypeMap.ext_var
 def VarTypeMap.ext_tvar
   (σ : VarTypeMap Γ Δ g) S :
   VarTypeMap (Ctx.extend_tvar Γ S) (Ctx.extend_tvar Δ (S.tsubst g)) g.ext_tvar := by
-  intros X S h
+  intros X S r h
   cases h
   case there_tvar =>
     rw [CType.tsubst_weaken_tvar_comm]
@@ -88,7 +155,7 @@ def VarTypeMap.ext_tvar
 
 def TVarSubst.ext_var
   (δ : TVarSubst Γ Δ g) P :
-  TVarSubst (Ctx.extend_var Γ P) (Ctx.extend_var Δ (P.tsubst g)) g.ext_var := by
+  TVarSubst (Ctx.extend_var Γ P p) (Ctx.extend_var Δ (P.tsubst g) p) g.ext_var := by
   intros X S h
   cases h
   case there_var h0 =>
@@ -122,39 +189,59 @@ def TVarSubst.ext_tvar
 
 def VarSubst.ext_tvar (σ : VarSubst Γ Δ f) R :
   VarSubst (Ctx.extend_tvar Γ R) (Ctx.extend_tvar Δ (R.rename f id)) f := by
-  intros X T h
+  intros X T r h
   cases h
   case there_tvar h =>
-    conv =>
-      arg 2
-      simp [VarMap.ext]
-    conv =>
-      arg 3
-      simp [VarMap.ext]
-    rw [<- id_ext]
-    rw [<- CType.rename_weaken_tvar_comm]
-    have h' := σ h
-    have h'' := h'.weaken_tvar (R.rename f id)
-    exact h''
+    apply And.intro
+    · conv =>
+        arg 2
+        simp [VarMap.ext]
+      conv =>
+        arg 3
+        simp [VarMap.ext]
+      rw [<- id_ext]
+      rw [<- CType.rename_weaken_tvar_comm]
+      have ⟨h', _⟩ := σ h
+      have h'' := h'.weaken_tvar (R.rename f id)
+      exact h''
+    · simp [ext_succ]
+      have ⟨_, h'⟩ := σ h
+      have h'' := h'.weaken_tvar (R.rename f id)
+      exact h''
 
-def VarSubst.open_var {Γ : Ctx n m} {y : Fin n} (h : Typed Γ (Term.var y) {y} P) :
-  VarSubst (Ctx.extend_var Γ P) Γ (open_map y) := by
+def VarSubst.open_var {Γ : Ctx n m} {y : Fin n}
+  (h : Typed Γ (Term.var y) {y} P)
+  (hs : SubcaptR Γ p ⟨∅, {y}, false⟩) :
+  VarSubst (Ctx.extend_var Γ P p) Γ (open_map y) := by
   unfold VarSubst
-  intros x T hb
+  intros x T r hb
   cases hb
   case here =>
-    simp
-    unfold CType.weaken_var
-    simp [CType.rename_comp]
-    trivial
+    apply And.intro
+    case left =>
+      simp
+      unfold CType.weaken_var
+      simp [CType.rename_comp]
+      trivial
+    case right =>
+      simp
+      unfold Region.weaken_var
+      simp [Region.rename_comp]
+      trivial
   case there_var =>
-    simp
-    unfold CType.weaken_var
-    simp [CType.rename_comp]
-    apply Typed.var_bound_type; aesop
+    apply And.intro
+    case left =>
+      simp
+      unfold CType.weaken_var
+      simp [CType.rename_comp]
+      apply Typed.var_bound_type; aesop
+    case right =>
+      simp
+      unfold Region.weaken_var; simp [Region.rename_comp]
+      apply SubcaptR.from_bound_var; trivial
 
 def TVarRename.open_var (h : Typed Γ (Term.var y) {y} P) :
-  TVarRename (Ctx.extend_var Γ P) Γ (open_map y) id := by
+  TVarRename (Ctx.extend_var Γ P p) Γ (open_map y) id := by
   unfold TVarRename
   intros X S h
   cases h
