CC/StoreContext/Basic.lean
@@ -16,30 +16,50 @@ namespace CC
 
 theorem lookup_store_typing
   (hs : TypedStore γ Γ)
-  (hx : BoundVar Γ x T)
+  (hx : BoundVar Γ x T r)
   (hl : LookupStore γ x v) :
   ∃ C, Typed Γ v.t C T := by
   induction hl
   case here =>
     cases hs
-    simp [Val.weaken_var]
-    cases hx
-    rename_i C T _ h _
-    have h' := h.weaken_var T
-    apply Exists.intro
-    apply h'
+    case cons =>
+      simp [Val.weaken_var]
+      cases hx
+      rename_i C T _ _ _ h
+      have h' := h.weaken_var T (Region.var 0)
+      apply Exists.intro
+      apply h'
+    case cons_empty =>
+      simp [Val.weaken_var]
+      cases hx
+      rename_i C T _ _ _ h
+      have h' := h.weaken_var T Region.glob
+      apply Exists.intro
+      apply h'
   case there ih =>
     cases hs
-    rename_i hs
-    have hx' := BoundVar.pred hx
-    let ⟨T0, ⟨hx1, hx2⟩⟩ := hx'
-    clear hx'
-    subst_vars
-    have ih' := ih hs hx2
-    cases ih'
-    constructor
-    apply Typed.weaken_var
-    aesop
+    case cons =>
+      rename_i hs _ _ _ _
+      have hx' := BoundVar.pred hx
+      let ⟨T0, r0, ⟨hx1, hx0, hx2⟩⟩ := hx'
+      clear hx'
+      subst_vars
+      have ih' := ih hs hx2
+      cases ih'
+      constructor
+      apply Typed.weaken_var
+      aesop
+    case cons_empty =>
+      rename_i hs _ _ _ _
+      have hx' := BoundVar.pred hx
+      let ⟨T0, r0, ⟨hx1, hx0, hx2⟩⟩ := hx'
+      clear hx'
+      subst_vars
+      have ih' := ih hs hx2
+      cases ih'
+      constructor
+      apply Typed.weaken_var
+      aesop
 
 lemma lookup_store_exists (γ : Store n) (x : Fin n) :
   ∃ v, LookupStore γ x v := by
@@ -48,6 +68,6 @@ lemma lookup_store_exists (γ : Store n) (x : Fin n) :
   case cons γ v ih =>
     cases x using Fin.cases with
     | H0 => constructor; constructor
-    | Hs x0 => 
+    | Hs x0 =>
       have ih' := ih x0; cases ih'
       constructor; constructor; assumption
