CC/Typed/Basic.lean
@@ -143,16 +143,16 @@ def LetHole1
   (Γ : Ctx n m)
   (u : Term n.succ m)
   (T : CType n m) (U : CType n m) : Prop :=
-  ∀ Ct' t' P,
-    Typed (Ctx.extend_var Γ P) t' Ct' T.weaken_var ->
-    ∃ C', Typed (Ctx.extend_var Γ P) (Term.letval t' u.weaken_var1) C' U.weaken_var
+  ∀ Ct' t' P p,
+    Typed (Ctx.extend_var Γ P p) t' Ct' T.weaken_var ->
+    ∃ C', Typed (Ctx.extend_var Γ P p) (Term.letval t' u.weaken_var1) C' U.weaken_var
 
 theorem Typed.let_inv' :
   t0 = Term.letval t u ->
   Typed Γ t0 C0 U ->
   ∃ Ct Cu T U0 U1,
     Typed Γ t Ct T ∧
-    Typed (Ctx.extend_var Γ T) u Cu U0 ∧
+    Typed (Ctx.extend_var Γ T Region.glob) u Cu U0 ∧
     U0 = CType.weaken_var U1 ∧
     Subtype Γ U1 U ∧
     LetHole Γ u T U ∧
@@ -167,10 +167,11 @@ theorem Typed.let_inv' :
     · intros Ct' t' Ht'
       constructor
       apply Typed.letval1 <;> try assumption
-    · intros Ct' t' P Ht'
+    · intros Ct' t' P p Ht'
       apply Exists.intro
       apply Typed.letval1
       exact Ht'
+      rw [<- Region.weaken_var_glob_def]
       apply Typed.weaken_var1
       trivial
       subst_vars
@@ -191,10 +192,11 @@ theorem Typed.let_inv' :
       assumption
       constructor
       assumption
-    · intros Ct' t' P Ht'
+    · intros Ct' t' P p Ht'
       apply Exists.intro
       apply Typed.letval1
       exact Ht'
+      rw [<- Region.weaken_var_glob_def]
       apply Typed.weaken_var1
       trivial
       subst_vars
@@ -215,8 +217,8 @@ theorem Typed.let_inv' :
       have ⟨C', h0⟩ := hh Ct' t' Ht'
       apply Exists.intro
       apply Typed.sub <;> trivial
-    · intros Ct' t' P Ht'
-      have ⟨C', h0⟩ := hh1 Ct' t' P Ht'
+    · intros Ct' t' P p Ht'
+      have ⟨C', h0⟩ := hh1 Ct' t' P p Ht'
       apply Exists.intro
       apply Typed.sub
       · trivial
@@ -226,7 +228,7 @@ theorem Typed.let_inv :
   Typed Γ (Term.letval t u) C0 U ->
   ∃ Ct Cu T U0 U1,
     Typed Γ t Ct T ∧
-    Typed (Ctx.extend_var Γ T) u Cu U0 ∧
+    Typed (Ctx.extend_var Γ T Region.glob) u Cu U0 ∧
     U0 = CType.weaken_var U1 ∧
     Subtype Γ U1 U ∧
     LetHole Γ u T U ∧ LetHole1 Γ u T U := by
@@ -249,7 +251,7 @@ theorem Typed.var_typing_bound' :
   t0 = Term.var x ->
   T0 = CType.capt C S ->
   Typed Γ t0 Cx T0 ->
-  ∃ C' S', BoundVar Γ x (CType.capt C' S') ∧ RSubtype Γ x S' S := by
+  ∃ C' S' r, BoundVar Γ x (CType.capt C' S') r ∧ RSubtype Γ x S' S := by
   intro he1 he2 h
   induction h <;> try (solve | cases he1 | cases he2)
   case var hb =>
@@ -261,7 +263,7 @@ theorem Typed.var_typing_bound' :
   case var_refine hr ih =>
     cases he1; cases he2
     have ih := ih rfl rfl
-    let ⟨C', S', hb, hsub⟩ := ih
+    let ⟨C', S', r, hb, hsub⟩ := ih
     repeat (apply Exists.intro)
     apply And.intro
     exact hb
@@ -272,7 +274,7 @@ theorem Typed.var_typing_bound' :
     cases he1; cases he2
     cases T
     have ih := ih rfl rfl
-    let ⟨C', S, hb, hsub0⟩ := ih
+    let ⟨C', S, r, hb, hsub0⟩ := ih
     repeat (apply Exists.intro)
     apply And.intro
     exact hb
@@ -283,7 +285,7 @@ theorem Typed.var_typing_bound' :
 
 theorem Typed.var_typing_bound :
   Typed Γ (Term.var x) Cx (CType.capt C S) ->
-  ∃ C' S', BoundVar Γ x (CType.capt C' S') ∧ RSubtype Γ x S' S := by
+  ∃ C' S' r, BoundVar Γ x (CType.capt C' S') r ∧ RSubtype Γ x S' S := by
   apply Typed.var_typing_bound' <;> aesop
 
 theorem Typed.var_typing_captures'
